Added level bounds...

DLCF/Syntax/BSubst.lean
@@ -4,17 +4,19 @@ namespace DLCF
 
 namespace Term
 
-def BSubst := ℕ → Term
+variable {Λ}
 
-def b0 (t : Term) : BSubst
+def BSubst (Λ) := ℕ → Term Λ
+
+def b0 (t : Term Λ) : BSubst Λ
   | 0 => t
   | n + 1 => .bound n
 
-def BSubst.lift (σ : BSubst) : BSubst
+def BSubst.lift (σ : BSubst Λ) : BSubst Λ
   | 0 => bound 0
   | n + 1 => (σ n).wk0
 
-def bsubst (σ : BSubst) : Term → Term
+def bsubst (σ : BSubst Λ) : Term Λ → Term Λ
   | bound n => σ n
   | univ n => univ n
   | epsilon A => epsilon (A.bsubst σ)
@@ -34,81 +36,81 @@ def bsubst (σ : BSubst) : Term → Term
   | qrec f => qrec (f.bsubst σ)
   | t => t
 
-def BSubst.id : BSubst := .bound
+def BSubst.id : BSubst Λ := .bound
 
 @[simp]
-theorem BSubst.lift_id : BSubst.id.lift = BSubst.id
+theorem BSubst.lift_id : BSubst.id.lift = BSubst.id (Λ := Λ)
   := funext (λn => by cases n <;> simp [id, lift, wk0, wk])
 
 @[simp]
-theorem BSubst.id_applied (n : ℕ) : BSubst.id n = bound n := rfl
+theorem BSubst.id_applied (n : ℕ) : BSubst.id (Λ := Λ) n = bound n := rfl
 
 @[simp]
-theorem bsubst_id (t : Term) : t.bsubst BSubst.id = t := by induction t <;> simp [bsubst, *]
+theorem bsubst_id (t : Term Λ) : t.bsubst BSubst.id = t := by induction t <;> simp [bsubst, *]
 
-def BSubst.comp (σ τ : BSubst) : BSubst := λn => (τ n).bsubst σ
-
-@[simp]
-theorem BSubst.comp_id (σ : BSubst) : σ.comp id = σ :=  rfl
+def BSubst.comp (σ τ : BSubst Λ) : BSubst Λ := λn => (τ n).bsubst σ
 
 @[simp]
-theorem BSubst.id_comp (σ : BSubst) : id.comp σ = σ := funext (λn => by simp [comp])
-
-def BSubst.ofWk (ρ : ℕ → ℕ) : BSubst := bound ∘ ρ
+theorem BSubst.comp_id (σ : BSubst Λ) : σ.comp id = σ :=  rfl
 
 @[simp]
-theorem BSubst.ofWk_applied (ρ : ℕ → ℕ) (n : ℕ) : (BSubst.ofWk ρ) n = bound (ρ n) := rfl
+theorem BSubst.id_comp (σ : BSubst Λ) : id.comp σ = σ := funext (λn => by simp [comp])
 
-theorem BSubst.ofWk_id : ofWk _root_.id = id := rfl
-
-theorem BSubst.ofWk_comp (ρ ρ' : ℕ → ℕ) : ofWk (ρ ∘ ρ') = (ofWk ρ).comp (ofWk ρ') := rfl
+def BSubst.ofWk (ρ : ℕ → ℕ) : BSubst Λ := bound ∘ ρ
 
 @[simp]
-theorem b0_comp_wk0 (t : Term) : t.b0.comp (BSubst.ofWk .succ) = BSubst.id
+theorem BSubst.ofWk_applied (ρ : ℕ → ℕ) (n : ℕ) : (BSubst.ofWk (Λ := Λ) ρ) n = bound (ρ n) := rfl
+
+theorem BSubst.ofWk_id : ofWk _root_.id = id (Λ := Λ) := rfl
+
+theorem BSubst.ofWk_comp (ρ ρ' : ℕ → ℕ) : ofWk (Λ := Λ) (ρ ∘ ρ') = (ofWk ρ).comp (ofWk ρ') := rfl
+
+@[simp]
+theorem b0_comp_wk0 (t : Term Λ) : t.b0.comp (BSubst.ofWk .succ) = BSubst.id
   := by funext k; cases k <;> rfl
 
-abbrev BSubst.wkIn (ρ : ℕ → ℕ) (σ : BSubst) : BSubst := σ ∘ ρ
+abbrev BSubst.wkIn (ρ : ℕ → ℕ) (σ : BSubst Λ) : BSubst Λ := σ ∘ ρ
 
-abbrev BSubst.wkOut (ρ : ℕ → ℕ) (σ : BSubst) : BSubst := (λn => (σ n).wk ρ)
+abbrev BSubst.wkOut (ρ : ℕ → ℕ) (σ : BSubst Λ) : BSubst Λ := (λn => (σ n).wk ρ)
 
-theorem BSubst.lift_wkIn (σ : BSubst) (ρ : ℕ → ℕ)
+theorem BSubst.lift_wkIn (σ : BSubst Λ) (ρ : ℕ → ℕ)
   : (σ.wkIn ρ).lift = σ.lift.wkIn (Nat.liftWk ρ) := funext (λn => by cases n <;> rfl)
 
-theorem bsubst_wkIn (σ : BSubst) (ρ : ℕ → ℕ) (t : Term)
+theorem bsubst_wkIn (σ : BSubst Λ) (ρ : ℕ → ℕ) (t : Term Λ)
   : t.bsubst (σ.wkIn ρ) = (t.wk ρ).bsubst σ
   := by induction t generalizing σ ρ <;> simp [bsubst, BSubst.lift_wkIn, *]
 
-theorem BSubst.lift_wkOut (σ : BSubst) (ρ : ℕ → ℕ)
+theorem BSubst.lift_wkOut (σ : BSubst Λ) (ρ : ℕ → ℕ)
   : (σ.wkOut ρ).lift = σ.lift.wkOut (Nat.liftWk ρ) := funext (λn =>
   by cases n <;> simp [wkOut, Nat.liftWk, lift, wk, wk0, <-wk_comp, Nat.liftWk_comp_succ])
 
-theorem bsubst_wkOut (σ : BSubst) (ρ : ℕ → ℕ) (t : Term)
+theorem bsubst_wkOut (σ : BSubst Λ) (ρ : ℕ → ℕ) (t : Term Λ)
   : t.bsubst (σ.wkOut ρ) = (t.bsubst σ).wk ρ
   := by induction t generalizing σ ρ <;> simp [bsubst, wk, BSubst.lift_wkOut, *]
 
-abbrev BSubst.wkIn0 := wkIn .succ
+abbrev BSubst.wkIn0 := wkIn (Λ := Λ) .succ
 
-abbrev BSubst.wkOut0 := wkOut .succ
+abbrev BSubst.wkOut0 := wkOut (Λ := Λ) .succ
 
-theorem bsubst_wkIn0 (σ : BSubst) (t : Term) : t.bsubst (σ.wkIn0) = (t.wk0).bsubst σ
+theorem bsubst_wkIn0 (σ : BSubst Λ) (t : Term Λ) : t.bsubst (σ.wkIn0) = (t.wk0).bsubst σ
   := bsubst_wkIn σ .succ t
 
-theorem bsubst_wkOut0 (σ : BSubst) (t : Term) : t.bsubst (σ.wkOut0) = (t.bsubst σ).wk0
+theorem bsubst_wkOut0 (σ : BSubst Λ) (t : Term Λ) : t.bsubst (σ.wkOut0) = (t.bsubst σ).wk0
   := bsubst_wkOut σ .succ t
 
-theorem BSubst.wkIn0_lift (σ : BSubst) : σ.lift.wkIn0 = σ.wkOut0
+theorem BSubst.wkIn0_lift (σ : BSubst Λ) : σ.lift.wkIn0 = σ.wkOut0
   := funext (λn => by cases n <;> rfl)
 
-theorem BSubst.lift_comp (σ τ : BSubst) : (σ.comp τ).lift = σ.lift.comp τ.lift := funext (λn
+theorem BSubst.lift_comp (σ τ : BSubst Λ) : (σ.comp τ).lift = σ.lift.comp τ.lift := funext (λn
   => by cases n <;> simp [bsubst, comp, lift, <-bsubst_wkIn0, <-bsubst_wkOut0, BSubst.wkIn0_lift])
 
-theorem bsubst_comp (σ τ : BSubst) (t : Term) : t.bsubst (σ.comp τ) = (t.bsubst τ).bsubst σ
+theorem bsubst_comp (σ τ : BSubst Λ) (t : Term Λ) : t.bsubst (σ.comp τ) = (t.bsubst τ).bsubst σ
   := by induction t generalizing σ τ <;> simp [bsubst, BSubst.comp, BSubst.lift_comp, *]
 
-theorem BSubst.comp_assoc (σ τ ρ : BSubst) : (σ.comp τ).comp ρ = σ.comp (τ.comp ρ) := funext (λn
+theorem BSubst.comp_assoc (σ τ ρ : BSubst Λ) : (σ.comp τ).comp ρ = σ.comp (τ.comp ρ) := funext (λn
   => by simp [BSubst.comp, bsubst_comp, *])
 
-instance BSubst.instMonoid : Monoid BSubst where
+instance BSubst.instMonoid : Monoid (BSubst Λ) where
   one := id
   mul := comp
   mul_assoc := comp_assoc
@@ -116,35 +118,35 @@ instance BSubst.instMonoid : Monoid BSubst where
   mul_one := comp_id
 
 @[simp]
-theorem BSubst.lift_one : (1 : BSubst).lift = 1 := BSubst.lift_id
+theorem BSubst.lift_one : (1 : BSubst Λ).lift = 1 := BSubst.lift_id
 
 @[simp]
-theorem BSubst.one_applied (n : ℕ) : (1 : BSubst) n = bound n := rfl
+theorem BSubst.one_applied (n : ℕ) : (1 : BSubst Λ) n = bound n := rfl
 
 @[simp]
-theorem bsubst_one (t : Term) : t.bsubst 1 = t := bsubst_id t
+theorem bsubst_one (t : Term Λ) : t.bsubst 1 = t := bsubst_id t
 
-theorem BSubst.lift_mul (σ τ : BSubst) : (σ * τ).lift = σ.lift * τ.lift := BSubst.lift_comp σ τ
+theorem BSubst.lift_mul (σ τ : BSubst Λ) : (σ * τ).lift = σ.lift * τ.lift := BSubst.lift_comp σ τ
 
-theorem bsubst_mul (σ τ : BSubst) (t : Term) : t.bsubst (σ * τ) = (t.bsubst τ).bsubst σ
+theorem bsubst_mul (σ τ : BSubst Λ) (t : Term Λ) : t.bsubst (σ * τ) = (t.bsubst τ).bsubst σ
   := bsubst_comp σ τ t
 
-instance mulActionBSubst : MulAction BSubst Term where
+instance mulActionBSubst : MulAction (BSubst Λ) (Term Λ) where
   smul := bsubst
   one_smul := bsubst_one
   mul_smul := bsubst_mul
 
-theorem BSubst.lift_ofWk (ρ : ℕ → ℕ) : (BSubst.ofWk ρ).lift = BSubst.ofWk (Nat.liftWk ρ)
+theorem BSubst.lift_ofWk (ρ : ℕ → ℕ) : (BSubst.ofWk ρ).lift (Λ := Λ) = BSubst.ofWk (Nat.liftWk ρ)
   := by funext n; cases n <;> rfl
 
-theorem bsubst_ofWk (ρ : ℕ → ℕ) (t : Term) : t.bsubst (BSubst.ofWk ρ) = t.wk ρ
+theorem bsubst_ofWk (ρ : ℕ → ℕ) (t : Term Λ) : t.bsubst (BSubst.ofWk ρ) = t.wk ρ
   := by induction t generalizing ρ <;> simp [wk, bsubst, BSubst.lift_ofWk, *]
 
 @[simp]
-theorem bsubst0_wk0 (t s : Term) : t.wk0.bsubst s.b0 = t
+theorem bsubst0_wk0 (t s : Term Λ) : t.wk0.bsubst s.b0 = t
   := by simp [wk0, <-bsubst_ofWk, <-bsubst_comp]
 
-theorem ofWk_smul (ρ : ℕ → ℕ) (t : Term) : (BSubst.ofWk ρ) • t = ρ • t := bsubst_ofWk ρ t
+theorem ofWk_smul (ρ : ℕ → ℕ) (t : Term Λ) : (BSubst.ofWk (Λ := Λ) ρ) • t = ρ • t := bsubst_ofWk ρ t
 
 -- TODO: class-ify?
 -- theorem bv_wk_le (ρ : ℕ → ℕ) (t : Term) (k : ℕ) (h : BoundedOn t.bv k ρ)
@@ -158,7 +160,7 @@ theorem ofWk_smul (ρ : ℕ → ℕ) (t : Term) : (BSubst.ofWk ρ) • t = ρ �
 --     sorry
 
 -- TODO: class-ify?
-def BSubst.BoundedOn (src trg : ℕ) (σ : BSubst) : Prop := ∀i ≤ src, (σ i).bv ≤ trg
+def BSubst.BoundedOn (src trg : ℕ) (σ : BSubst Λ) : Prop := ∀i ≤ src, (σ i).bv ≤ trg
 
 -- theorem bv_bsubst_le (σ : BSubst) (t : Term) (k : ℕ) (h : ∀i < t.bv, (σ i).bv ≤ k)
 --   : (t.bsubst σ).bv ≤ k := by
