DLCF/Syntax/FSubst.lean
@@ -4,42 +4,44 @@ namespace DLCF
 
 namespace Term
 
-def FSubst := FVar → Term
+variable {Λ}
 
-def FSubst.wk (ρ : ℕ → ℕ) (σ : FSubst) : FSubst := λx => (σ x).wk ρ
+def FSubst (Λ) := FVar Λ → Term Λ
+
+def FSubst.wk (ρ : ℕ → ℕ) (σ : FSubst Λ) : FSubst Λ := λx => (σ x).wk ρ
 
 @[simp]
-theorem FSubst.wk_applied (ρ : ℕ → ℕ) (σ : FSubst)
+theorem FSubst.wk_applied (ρ : ℕ → ℕ) (σ : FSubst Λ)
   : (σ.wk ρ) x = (σ x).wk ρ := rfl
 
 @[simp]
-theorem FSubst.wk_id (σ : FSubst) : σ.wk id = σ := by funext x; simp
+theorem FSubst.wk_id (σ : FSubst Λ) : σ.wk id = σ := by funext x; simp
 
-theorem FSubst.wk_comp (ρ ρ' : ℕ → ℕ) (σ : FSubst)
+theorem FSubst.wk_comp (ρ ρ' : ℕ → ℕ) (σ : FSubst Λ)
   : σ.wk (ρ ∘ ρ') = (σ.wk ρ').wk ρ := by funext x; simp [Term.wk_comp]
 
-instance FSubst.wkSMul : SMul (ℕ → ℕ) FSubst where
+instance FSubst.wkSMul : SMul (ℕ → ℕ) (FSubst Λ) where
   smul := FSubst.wk
 
-theorem FSubst.smul_wk_def (ρ : ℕ → ℕ) (σ : FSubst) : ρ • σ = σ.wk ρ := rfl
+theorem FSubst.smul_wk_def (ρ : ℕ → ℕ) (σ : FSubst Λ) : ρ • σ = σ.wk ρ := rfl
 
 @[simp]
-theorem FSubst.smul_wk_applied (ρ : ℕ → ℕ) (σ : FSubst) (x)
+theorem FSubst.smul_wk_applied (ρ : ℕ → ℕ) (σ : FSubst Λ) (x)
   : (ρ • σ) x = ρ • σ x := rfl
 
 @[simp]
-theorem FSubst.id_smul_wk (σ : FSubst) : _root_.id (α := ℕ) • σ = σ :=  wk_id σ
+theorem FSubst.id_smul_wk (σ : FSubst Λ) : _root_.id (α := ℕ) • σ = σ :=  wk_id σ
 
-theorem FSubst.comp_smul_wk (ρ ρ' : ℕ → ℕ) (σ : FSubst)
+theorem FSubst.comp_smul_wk (ρ ρ' : ℕ → ℕ) (σ : FSubst Λ)
   : (ρ ∘ ρ') • σ = ρ • (ρ' • σ) := wk_comp ρ ρ' σ
 
-def FSubst.lift (σ : FSubst) : FSubst := σ.wk .succ
+def FSubst.lift (σ : FSubst Λ) : FSubst Λ := σ.wk .succ
 
 @[simp]
-theorem FSubst.lift_applied (σ : FSubst) (x)
+theorem FSubst.lift_applied (σ : FSubst Λ) (x)
   : σ.lift x = (σ x).wk0 := rfl
 
-def fsubst (σ : FSubst) : Term → Term
+def fsubst (σ : FSubst Λ) : Term Λ → Term Λ
   | free n A => σ ⟨n, A⟩
   | epsilon A => epsilon (A.fsubst σ)
   | dite c t f => dite (c.fsubst σ) (t.fsubst σ.lift) (f.fsubst σ.lift)
@@ -58,45 +60,45 @@ def fsubst (σ : FSubst) : Term → Term
   | qrec f => qrec (f.fsubst σ)
   | t => t
 
-def FSubst.id : FSubst := λx => .free x.name x.ty
+def FSubst.id : FSubst Λ := λx => .free x.name x.ty
 
 @[simp]
-theorem FSubst.lift_id : id.lift = id := rfl
+theorem FSubst.lift_id : id.lift (Λ := Λ) = id := rfl
 
 @[simp]
-theorem FSubst.id_applied (x) : id x = x := rfl
+theorem FSubst.id_applied (x) : id (Λ := Λ) x = x := rfl
 
 @[simp]
-theorem fsubst_id (t : Term) : t.fsubst FSubst.id = t := by
+theorem fsubst_id (t : Term Λ) : t.fsubst FSubst.id = t := by
   induction t <;> simp [fsubst, *]
 
-theorem wk_fsubst  (ρ : ℕ → ℕ) (σ : FSubst) (t : Term)
+theorem wk_fsubst  (ρ : ℕ → ℕ) (σ : FSubst Λ) (t : Term Λ)
   : (t.fsubst σ).wk ρ = (t.wk ρ).fsubst (σ.wk ρ) := by
   induction t generalizing ρ σ
   <;> simp [wk, fsubst, FSubst.lift, <-FSubst.wk_comp, Nat.liftWk_comp_succ, *]
 
-def FSubst.comp (σ τ : FSubst) : FSubst := λx => (τ x).fsubst σ
+def FSubst.comp (σ τ : FSubst Λ) : FSubst Λ := λx => (τ x).fsubst σ
 
 @[simp]
-theorem FSubst.comp_applied (σ τ : FSubst) (x)
+theorem FSubst.comp_applied (σ τ : FSubst Λ) (x)
   : (σ.comp τ) x = (τ x).fsubst σ := rfl
 
-@[simp] theorem FSubst.comp_id (σ : FSubst) : σ.comp id = σ := rfl
+@[simp] theorem FSubst.comp_id (σ : FSubst Λ) : σ.comp id = σ := rfl
 
-@[simp] theorem FSubst.id_comp (σ : FSubst) : id.comp σ = σ := by funext x; simp [comp]
+@[simp] theorem FSubst.id_comp (σ : FSubst Λ) : id.comp σ = σ := by funext x; simp [comp]
 
-theorem FSubst.comp_wk (ρ : ℕ → ℕ) (σ τ : FSubst)
+theorem FSubst.comp_wk (ρ : ℕ → ℕ) (σ τ : FSubst Λ)
   : (σ.comp τ).wk ρ = (σ.wk ρ).comp (τ.wk ρ) := by funext x; simp [comp, wk_fsubst, *]
 
-theorem FSubst.lift_comp (σ τ : FSubst) : (σ.comp τ).lift = σ.lift.comp τ.lift := comp_wk .succ σ τ
+theorem FSubst.lift_comp (σ τ : FSubst Λ) : (σ.comp τ).lift = σ.lift.comp τ.lift := comp_wk .succ σ τ
 
-theorem fsubst_comp (σ τ : FSubst) (t : Term) : t.fsubst (σ.comp τ) = (t.fsubst τ).fsubst σ
+theorem fsubst_comp (σ τ : FSubst Λ) (t : Term Λ) : t.fsubst (σ.comp τ) = (t.fsubst τ).fsubst σ
   := by induction t generalizing σ τ <;> simp [fsubst, FSubst.lift_comp, *]
 
-theorem FSubst.comp_assoc (σ τ ρ : FSubst) : (σ.comp τ).comp ρ = σ.comp (τ.comp ρ) := by
+theorem FSubst.comp_assoc (σ τ ρ : FSubst Λ) : (σ.comp τ).comp ρ = σ.comp (τ.comp ρ) := by
   funext x; simp [FSubst.comp, fsubst_comp, *]
 
-instance FSubst.instMonoid : Monoid FSubst where
+instance FSubst.instMonoid : Monoid (FSubst Λ) where
   one := id
   mul := comp
   one_mul := FSubst.id_comp
@@ -104,48 +106,23 @@ instance FSubst.instMonoid : Monoid FSubst where
   mul_assoc := FSubst.comp_assoc
 
 @[simp]
-theorem FSubst.one_applied (x) : (1 : FSubst) x = x := rfl
+theorem FSubst.one_applied (x) : (1 : FSubst Λ) x = x := rfl
 
-theorem fsubst_one (t : Term) : t.fsubst 1 = t := fsubst_id t
+theorem fsubst_one (t : Term Λ) : t.fsubst 1 = t := fsubst_id t
 
-theorem fsubst_mul (σ τ : FSubst) (t : Term)
+theorem fsubst_mul (σ τ : FSubst Λ) (t : Term Λ)
   : t.fsubst (σ * τ) = (t.fsubst τ).fsubst σ := fsubst_comp σ τ t
 
-instance mulActionFSubst : MulAction FSubst Term where
+instance mulActionFSubst : MulAction (FSubst Λ) (Term Λ) where
   smul := fsubst
   one_smul := fsubst_one
   mul_smul := fsubst_mul
 
-theorem FSubst.lift_one : (1 : FSubst).lift = 1 := FSubst.lift_id
+theorem FSubst.lift_one : (1 : FSubst Λ).lift = 1 := FSubst.lift_id
 
-theorem FSubst.lift_mul (σ τ : FSubst) : (σ * τ).lift = σ.lift * τ.lift := FSubst.lift_comp σ τ
+theorem FSubst.lift_mul (σ τ : FSubst Λ) : (σ * τ).lift = σ.lift * τ.lift := FSubst.lift_comp σ τ
 
-def FSubst.set (σ : FSubst) (x : FVar) (a : Term) : FSubst
-  := Function.update σ x a
-
-@[simp]
-theorem FSubst.set_same (σ : FSubst) (x) (a : Term)
-  : (σ.set x a) x = a := by simp [set]
-
-@[simp]
-theorem FSubst.set_idem (σ : FSubst) (a b : Term)
-  : (σ.set x a).set x b = σ.set x b := by simp [set]
-
-theorem FSubst.wk_set (ρ : ℕ → ℕ) (σ : FSubst) (x) (a : Term)
-  : (σ.set x a).wk ρ = (σ.wk ρ).set x (a.wk ρ) := by
-  funext y; simp only [set, wk_applied, Function.update, eq_rec_constant, dite_eq_ite]
-  split <;> rfl
-
-theorem FSubst.smul_wk_set (ρ : ℕ → ℕ) (σ : FSubst) (x) (a : Term)
-  : ρ • (σ.set x a) = (ρ • σ).set x (a.wk ρ)
-  := wk_set ρ σ x a
-
-theorem FSubst.lift_set (σ : FSubst) (x) (a : Term)
-  : (σ.set x a).lift = σ.lift.set x a.wk0 := wk_set .succ σ x a
-
-def fset (t : Term) (x : FVar) (a : Term) : Term := t.fsubst (FSubst.id.set x a)
-
-theorem FSubst.free_on_lift_iff {σ : FSubst} {V : Finset FVar}
+theorem FSubst.free_on_lift_iff {σ : FSubst Λ} {V : Finset (FVar Λ)}
   : (∀x ∈ V, σ.lift x = x) ↔ (∀x ∈ V, σ x = x)
   := by
   rw [forall_congr]
@@ -155,10 +132,37 @@ theorem FSubst.free_on_lift_iff {σ : FSubst} {V : Finset FVar}
   generalize σ x = s
   cases s <;> simp [Term.wk]
 
-theorem FSubst.free_on_lift {σ : FSubst} {V : Finset FVar} (h : ∀x ∈ V, σ x = x)
+theorem FSubst.free_on_lift {σ : FSubst Λ} {V : Finset (FVar Λ)} (h : ∀x ∈ V, σ x = x)
   : ∀x ∈ V, σ.lift x = x := free_on_lift_iff.mpr h
 
-theorem fsubst_id_on (σ : FSubst) (t : Term) (h : ∀x ∈ t.fv, σ x = x)
+variable [DecidableEq Λ]
+
+def FSubst.set (σ : FSubst Λ) (x : FVar Λ) (a : Term Λ) : FSubst Λ
+  := Function.update σ x a
+
+@[simp]
+theorem FSubst.set_same (σ : FSubst Λ) (x) (a : Term Λ)
+  : (σ.set x a) x = a := by simp [set]
+
+@[simp]
+theorem FSubst.set_idem (σ : FSubst Λ) (a b : Term Λ)
+  : (σ.set x a).set x b = σ.set x b := by simp [set]
+
+theorem FSubst.wk_set (ρ : ℕ → ℕ) (σ : FSubst Λ) (x) (a : Term Λ)
+  : (σ.set x a).wk ρ = (σ.wk ρ).set x (a.wk ρ) := by
+  funext y; simp only [set, wk_applied, Function.update, eq_rec_constant, dite_eq_ite]
+  split <;> rfl
+
+theorem FSubst.smul_wk_set (ρ : ℕ → ℕ) (σ : FSubst Λ) (x) (a : Term Λ)
+  : ρ • (σ.set x a) = (ρ • σ).set x (a.wk ρ)
+  := wk_set ρ σ x a
+
+theorem FSubst.lift_set (σ : FSubst Λ) (x) (a : Term Λ)
+  : (σ.set x a).lift = σ.lift.set x a.wk0 := wk_set .succ σ x a
+
+def fset (t : Term Λ) (x : FVar Λ) (a : Term Λ) : Term Λ := t.fsubst (FSubst.id.set x a)
+
+theorem fsubst_id_on (σ : FSubst Λ) (t : Term Λ) (h : ∀x ∈ t.fv, σ x = x)
   : t.fsubst σ = t := by induction t generalizing σ with
   | free n A => exact h ⟨n, A⟩ (by simp [fv])
   | _ =>
