DLCF/Syntax/Subst.lean
@@ -5,26 +5,28 @@ namespace DLCF
 
 namespace Term
 
-def FSubst.bsubst (τ : BSubst) (σ : FSubst) : FSubst := λx => τ • (σ x)
+variable {Λ}
+
+def FSubst.bsubst (τ : BSubst Λ) (σ : FSubst Λ) : FSubst Λ := λx => τ • (σ x)
 
 @[simp]
-theorem FSubst.bsubst_applied (τ : BSubst) (σ : FSubst) (x)
+theorem FSubst.bsubst_applied (τ : BSubst Λ) (σ : FSubst Λ) (x)
   : (σ.bsubst τ) x = τ • (σ x) := rfl
 
 @[simp]
-theorem FSubst.bsubst_one (σ : FSubst) : σ.bsubst 1 = σ := by funext x; simp
+theorem FSubst.bsubst_one (σ : FSubst Λ) : σ.bsubst 1 = σ := by funext x; simp
 
-theorem FSubst.bsubst_mul (τ ρ : BSubst) (σ : FSubst) : (σ.bsubst (τ * ρ)) = (σ.bsubst ρ).bsubst τ
+theorem FSubst.bsubst_mul (τ ρ : BSubst Λ) (σ : FSubst Λ) : (σ.bsubst (τ * ρ)) = (σ.bsubst ρ).bsubst τ
   := by funext x; simp [mul_smul]
 
 @[simp]
-theorem FSubst.bsubst_id (σ : FSubst) : σ.bsubst BSubst.id = σ := bsubst_one σ
+theorem FSubst.bsubst_id (σ : FSubst Λ) : σ.bsubst BSubst.id = σ := bsubst_one σ
 
-theorem FSubst.bsubst_comp (τ ρ : BSubst) (σ : FSubst)
+theorem FSubst.bsubst_comp (τ ρ : BSubst Λ) (σ : FSubst Λ)
   : (σ.bsubst (τ.comp ρ)) = (σ.bsubst ρ).bsubst τ
   := bsubst_mul τ ρ σ
 
-instance FSubst.mulActionFSubst : MulAction BSubst FSubst where
+instance FSubst.mulActionFSubst : MulAction (BSubst Λ) (FSubst Λ) where
   smul := bsubst
   one_smul := bsubst_one
   mul_smul := bsubst_mul
